spec/haskell/src/SEL4/Kernel/Thread/ARM.lhs
@@ -17,13 +17,13 @@ This module contains the architecture-specific thread switch code for the ARM.
 > import SEL4.Machine
 > import SEL4.Machine.RegisterSet.ARM
 > import SEL4.Model.StateData
-> import SEL4.Model.StateData.ARM
+> -- import SEL4.Model.StateData.ARM
 > import SEL4.Object.Structures
 > import SEL4.Object.TCB
 > import SEL4.Kernel.VSpace.ARM
 > import qualified SEL4.Machine.Hardware.ARM as ARMHardware
 > import {-# SOURCE #-} SEL4.Kernel.Init
-> import SEL4.Model.PSpace
+> -- import SEL4.Model.PSpace
 
 \end{impdetails}
 
@@ -32,9 +32,8 @@ The ARM thread switch function invalidates all caches and the TLB, and writes th
 > switchToThread :: PPtr TCB -> Kernel ()
 > switchToThread tcb = do
 >     setVMRoot tcb
->     globals <- gets $ armKSGlobalsFrame . ksArchState
 >     bufferPtr <- threadGet tcbIPCBuffer tcb
->     storeWordUser globals $ fromVPtr bufferPtr
+>     asUser tcb $ setRegister (Register TPIDRURW) $ fromVPtr bufferPtr
 >     doMachineOp $ ARMHardware.clearExMonitor
 
 The ARM idle thread runs in system mode with interrupts enabled, with the PC pointing to a small kernel routine that executes a wait-for-interrupt instruction. In the Haskell model, this routine is placed in the globals page, so the simulator can access it; in a real kernel there would be no need for it to be user-accessible.
@@ -48,9 +47,7 @@ The ARM idle thread runs in system mode with interrupts enabled, with the PC poi
 Since the idle thread only accesses global mappings, there is nothing to be done when switching to it.
 
 > switchToIdleThread :: Kernel ()
-> switchToIdleThread = do
->  globals <- gets $ armKSGlobalsFrame . ksArchState
->  storeWordUser globals 0
+> switchToIdleThread = return ()
 
 There is nothing special about idle thread activation on ARM.
 
