proof/invariant-abstract/ARM/ArchAcc_AI.thy
@@ -601,8 +601,8 @@ lemma kernel_mapping_slots_empty_pdeI:
   apply (clarsimp simp: invs_def valid_state_def equal_kernel_mappings_def valid_global_objs_def)
   apply (erule_tac x=p in allE, erule_tac x="arm_global_pd (arch_state s)" in allE)
   including unfold_objects
-  by (clarsimp simp: empty_table_def valid_arch_state_def a_type_def)
-
+  apply clarsimp
+by (simp add: empty_table_def valid_arch_state_def a_type_def)
 
 lemma invs_valid_global_pts:
   "invs s \<Longrightarrow> valid_global_pts s"
