spec/design/API_H.thy
@@ -22,6 +22,7 @@ definition
 callKernel :: "event \<Rightarrow> unit kernel"
 where
 "callKernel ev\<equiv> (do
+    if (callHook ev) then cEntryHook else return ();
     runErrorT $ handleEvent ev
         `~catchError~` (\<lambda> _. withoutPreemption $ (do
                       irq \<leftarrow> doMachineOp getActiveIRQ;
@@ -29,7 +30,8 @@ where
         od)
                                                                         );
     schedule;
-    activateThread
+    activateThread;
+    if (callHook ev) then cExitHook else return ()
 od)"
 
 definition
