spec/design/ARM/ArchStateData_H.thy
@@ -25,223 +25,85 @@ begin
 context Arch begin global_naming ARM_H
 
 datatype kernel_state =
-    ARMKernelState machine_word "asid \<Rightarrow> ((machine_word) option)" "hardware_asid \<Rightarrow> (asid option)" hardware_asid "asid \<Rightarrow> ((hardware_asid * machine_word) option)" machine_word "machine_word list" "machine_word \<Rightarrow> arm_vspace_region_use"
-
-primrec
-  armKSGlobalsFrame :: "kernel_state \<Rightarrow> machine_word"
-where
-  "armKSGlobalsFrame (ARMKernelState v0 v1 v2 v3 v4 v5 v6 v7) = v0"
-
-primrec
-  armKSASIDTable :: "kernel_state \<Rightarrow> asid \<Rightarrow> ((machine_word) option)"
-where
-  "armKSASIDTable (ARMKernelState v0 v1 v2 v3 v4 v5 v6 v7) = v1"
-
-primrec
-  armKSGlobalPD :: "kernel_state \<Rightarrow> machine_word"
-where
-  "armKSGlobalPD (ARMKernelState v0 v1 v2 v3 v4 v5 v6 v7) = v5"
-
-primrec
-  armKSHWASIDTable :: "kernel_state \<Rightarrow> hardware_asid \<Rightarrow> (asid option)"
-where
-  "armKSHWASIDTable (ARMKernelState v0 v1 v2 v3 v4 v5 v6 v7) = v2"
+    ARMKernelState "asid \<Rightarrow> ((machine_word) option)" "hardware_asid \<Rightarrow> (asid option)" hardware_asid "asid \<Rightarrow> ((hardware_asid * machine_word) option)" machine_word "machine_word list" "machine_word \<Rightarrow> arm_vspace_region_use"
 
 primrec
   armKSKernelVSpace :: "kernel_state \<Rightarrow> machine_word \<Rightarrow> arm_vspace_region_use"
 where
-  "armKSKernelVSpace (ARMKernelState v0 v1 v2 v3 v4 v5 v6 v7) = v7"
+  "armKSKernelVSpace (ARMKernelState v0 v1 v2 v3 v4 v5 v6) = v6"
+
+primrec
+  armKSASIDTable :: "kernel_state \<Rightarrow> asid \<Rightarrow> ((machine_word) option)"
+where
+  "armKSASIDTable (ARMKernelState v0 v1 v2 v3 v4 v5 v6) = v0"
+
+primrec
+  armKSGlobalPD :: "kernel_state \<Rightarrow> machine_word"
+where
+  "armKSGlobalPD (ARMKernelState v0 v1 v2 v3 v4 v5 v6) = v4"
+
+primrec
+  armKSHWASIDTable :: "kernel_state \<Rightarrow> hardware_asid \<Rightarrow> (asid option)"
+where
+  "armKSHWASIDTable (ARMKernelState v0 v1 v2 v3 v4 v5 v6) = v1"
 
 primrec
   armKSGlobalPTs :: "kernel_state \<Rightarrow> machine_word list"
 where
-  "armKSGlobalPTs (ARMKernelState v0 v1 v2 v3 v4 v5 v6 v7) = v6"
+  "armKSGlobalPTs (ARMKernelState v0 v1 v2 v3 v4 v5 v6) = v5"
 
 primrec
   armKSNextASID :: "kernel_state \<Rightarrow> hardware_asid"
 where
-  "armKSNextASID (ARMKernelState v0 v1 v2 v3 v4 v5 v6 v7) = v3"
+  "armKSNextASID (ARMKernelState v0 v1 v2 v3 v4 v5 v6) = v2"
 
 primrec
   armKSASIDMap :: "kernel_state \<Rightarrow> asid \<Rightarrow> ((hardware_asid * machine_word) option)"
 where
-  "armKSASIDMap (ARMKernelState v0 v1 v2 v3 v4 v5 v6 v7) = v4"
-
-primrec
-  armKSGlobalsFrame_update :: "(machine_word \<Rightarrow> machine_word) \<Rightarrow> kernel_state \<Rightarrow> kernel_state"
-where
-  "armKSGlobalsFrame_update f (ARMKernelState v0 v1 v2 v3 v4 v5 v6 v7) = ARMKernelState (f v0) v1 v2 v3 v4 v5 v6 v7"
-
-primrec
-  armKSASIDTable_update :: "((asid \<Rightarrow> ((machine_word) option)) \<Rightarrow> (asid \<Rightarrow> ((machine_word) option))) \<Rightarrow> kernel_state \<Rightarrow> kernel_state"
-where
-  "armKSASIDTable_update f (ARMKernelState v0 v1 v2 v3 v4 v5 v6 v7) = ARMKernelState v0 (f v1) v2 v3 v4 v5 v6 v7"
-
-primrec
-  armKSGlobalPD_update :: "(machine_word \<Rightarrow> machine_word) \<Rightarrow> kernel_state \<Rightarrow> kernel_state"
-where
-  "armKSGlobalPD_update f (ARMKernelState v0 v1 v2 v3 v4 v5 v6 v7) = ARMKernelState v0 v1 v2 v3 v4 (f v5) v6 v7"
-
-primrec
-  armKSHWASIDTable_update :: "((hardware_asid \<Rightarrow> (asid option)) \<Rightarrow> (hardware_asid \<Rightarrow> (asid option))) \<Rightarrow> kernel_state \<Rightarrow> kernel_state"
-where
-  "armKSHWASIDTable_update f (ARMKernelState v0 v1 v2 v3 v4 v5 v6 v7) = ARMKernelState v0 v1 (f v2) v3 v4 v5 v6 v7"
+  "armKSASIDMap (ARMKernelState v0 v1 v2 v3 v4 v5 v6) = v3"
 
 primrec
   armKSKernelVSpace_update :: "((machine_word \<Rightarrow> arm_vspace_region_use) \<Rightarrow> (machine_word \<Rightarrow> arm_vspace_region_use)) \<Rightarrow> kernel_state \<Rightarrow> kernel_state"
 where
-  "armKSKernelVSpace_update f (ARMKernelState v0 v1 v2 v3 v4 v5 v6 v7) = ARMKernelState v0 v1 v2 v3 v4 v5 v6 (f v7)"
+  "armKSKernelVSpace_update f (ARMKernelState v0 v1 v2 v3 v4 v5 v6) = ARMKernelState v0 v1 v2 v3 v4 v5 (f v6)"
+
+primrec
+  armKSASIDTable_update :: "((asid \<Rightarrow> ((machine_word) option)) \<Rightarrow> (asid \<Rightarrow> ((machine_word) option))) \<Rightarrow> kernel_state \<Rightarrow> kernel_state"
+where
+  "armKSASIDTable_update f (ARMKernelState v0 v1 v2 v3 v4 v5 v6) = ARMKernelState (f v0) v1 v2 v3 v4 v5 v6"
+
+primrec
+  armKSGlobalPD_update :: "(machine_word \<Rightarrow> machine_word) \<Rightarrow> kernel_state \<Rightarrow> kernel_state"
+where
+  "armKSGlobalPD_update f (ARMKernelState v0 v1 v2 v3 v4 v5 v6) = ARMKernelState v0 v1 v2 v3 (f v4) v5 v6"
+
+primrec
+  armKSHWASIDTable_update :: "((hardware_asid \<Rightarrow> (asid option)) \<Rightarrow> (hardware_asid \<Rightarrow> (asid option))) \<Rightarrow> kernel_state \<Rightarrow> kernel_state"
+where
+  "armKSHWASIDTable_update f (ARMKernelState v0 v1 v2 v3 v4 v5 v6) = ARMKernelState v0 (f v1) v2 v3 v4 v5 v6"
 
 primrec
   armKSGlobalPTs_update :: "((machine_word list) \<Rightarrow> (machine_word list)) \<Rightarrow> kernel_state \<Rightarrow> kernel_state"
 where
-  "armKSGlobalPTs_update f (ARMKernelState v0 v1 v2 v3 v4 v5 v6 v7) = ARMKernelState v0 v1 v2 v3 v4 v5 (f v6) v7"
+  "armKSGlobalPTs_update f (ARMKernelState v0 v1 v2 v3 v4 v5 v6) = ARMKernelState v0 v1 v2 v3 v4 (f v5) v6"
 
 primrec
   armKSNextASID_update :: "(hardware_asid \<Rightarrow> hardware_asid) \<Rightarrow> kernel_state \<Rightarrow> kernel_state"
 where
-  "armKSNextASID_update f (ARMKernelState v0 v1 v2 v3 v4 v5 v6 v7) = ARMKernelState v0 v1 v2 (f v3) v4 v5 v6 v7"
+  "armKSNextASID_update f (ARMKernelState v0 v1 v2 v3 v4 v5 v6) = ARMKernelState v0 v1 (f v2) v3 v4 v5 v6"
 
 primrec
   armKSASIDMap_update :: "((asid \<Rightarrow> ((hardware_asid * machine_word) option)) \<Rightarrow> (asid \<Rightarrow> ((hardware_asid * machine_word) option))) \<Rightarrow> kernel_state \<Rightarrow> kernel_state"
 where
-  "armKSASIDMap_update f (ARMKernelState v0 v1 v2 v3 v4 v5 v6 v7) = ARMKernelState v0 v1 v2 v3 (f v4) v5 v6 v7"
+  "armKSASIDMap_update f (ARMKernelState v0 v1 v2 v3 v4 v5 v6) = ARMKernelState v0 v1 v2 (f v3) v4 v5 v6"
 
 abbreviation (input)
-  ARMKernelState_trans :: "(machine_word) \<Rightarrow> (asid \<Rightarrow> ((machine_word) option)) \<Rightarrow> (hardware_asid \<Rightarrow> (asid option)) \<Rightarrow> (hardware_asid) \<Rightarrow> (asid \<Rightarrow> ((hardware_asid * machine_word) option)) \<Rightarrow> (machine_word) \<Rightarrow> (machine_word list) \<Rightarrow> (machine_word \<Rightarrow> arm_vspace_region_use) \<Rightarrow> kernel_state" ("ARMKernelState'_ \<lparr> armKSGlobalsFrame= _, armKSASIDTable= _, armKSHWASIDTable= _, armKSNextASID= _, armKSASIDMap= _, armKSGlobalPD= _, armKSGlobalPTs= _, armKSKernelVSpace= _ \<rparr>")
+  ARMKernelState_trans :: "(asid \<Rightarrow> ((machine_word) option)) \<Rightarrow> (hardware_asid \<Rightarrow> (asid option)) \<Rightarrow> (hardware_asid) \<Rightarrow> (asid \<Rightarrow> ((hardware_asid * machine_word) option)) \<Rightarrow> (machine_word) \<Rightarrow> (machine_word list) \<Rightarrow> (machine_word \<Rightarrow> arm_vspace_region_use) \<Rightarrow> kernel_state" ("ARMKernelState'_ \<lparr> armKSASIDTable= _, armKSHWASIDTable= _, armKSNextASID= _, armKSASIDMap= _, armKSGlobalPD= _, armKSGlobalPTs= _, armKSKernelVSpace= _ \<rparr>")
 where
-  "ARMKernelState_ \<lparr> armKSGlobalsFrame= v0, armKSASIDTable= v1, armKSHWASIDTable= v2, armKSNextASID= v3, armKSASIDMap= v4, armKSGlobalPD= v5, armKSGlobalPTs= v6, armKSKernelVSpace= v7 \<rparr> == ARMKernelState v0 v1 v2 v3 v4 v5 v6 v7"
+  "ARMKernelState_ \<lparr> armKSASIDTable= v0, armKSHWASIDTable= v1, armKSNextASID= v2, armKSASIDMap= v3, armKSGlobalPD= v4, armKSGlobalPTs= v5, armKSKernelVSpace= v6 \<rparr> == ARMKernelState v0 v1 v2 v3 v4 v5 v6"
 
-lemma armKSGlobalsFrame_armKSGlobalsFrame_update [simp]:
-  "armKSGlobalsFrame (armKSGlobalsFrame_update f v) = f (armKSGlobalsFrame v)"
-  by (cases v) simp
-
-lemma armKSGlobalsFrame_armKSASIDTable_update [simp]:
-  "armKSGlobalsFrame (armKSASIDTable_update f v) = armKSGlobalsFrame v"
-  by (cases v) simp
-
-lemma armKSGlobalsFrame_armKSGlobalPD_update [simp]:
-  "armKSGlobalsFrame (armKSGlobalPD_update f v) = armKSGlobalsFrame v"
-  by (cases v) simp
-
-lemma armKSGlobalsFrame_armKSHWASIDTable_update [simp]:
-  "armKSGlobalsFrame (armKSHWASIDTable_update f v) = armKSGlobalsFrame v"
-  by (cases v) simp
-
-lemma armKSGlobalsFrame_armKSKernelVSpace_update [simp]:
-  "armKSGlobalsFrame (armKSKernelVSpace_update f v) = armKSGlobalsFrame v"
-  by (cases v) simp
-
-lemma armKSGlobalsFrame_armKSGlobalPTs_update [simp]:
-  "armKSGlobalsFrame (armKSGlobalPTs_update f v) = armKSGlobalsFrame v"
-  by (cases v) simp
-
-lemma armKSGlobalsFrame_armKSNextASID_update [simp]:
-  "armKSGlobalsFrame (armKSNextASID_update f v) = armKSGlobalsFrame v"
-  by (cases v) simp
-
-lemma armKSGlobalsFrame_armKSASIDMap_update [simp]:
-  "armKSGlobalsFrame (armKSASIDMap_update f v) = armKSGlobalsFrame v"
-  by (cases v) simp
-
-lemma armKSASIDTable_armKSGlobalsFrame_update [simp]:
-  "armKSASIDTable (armKSGlobalsFrame_update f v) = armKSASIDTable v"
-  by (cases v) simp
-
-lemma armKSASIDTable_armKSASIDTable_update [simp]:
-  "armKSASIDTable (armKSASIDTable_update f v) = f (armKSASIDTable v)"
-  by (cases v) simp
-
-lemma armKSASIDTable_armKSGlobalPD_update [simp]:
-  "armKSASIDTable (armKSGlobalPD_update f v) = armKSASIDTable v"
-  by (cases v) simp
-
-lemma armKSASIDTable_armKSHWASIDTable_update [simp]:
-  "armKSASIDTable (armKSHWASIDTable_update f v) = armKSASIDTable v"
-  by (cases v) simp
-
-lemma armKSASIDTable_armKSKernelVSpace_update [simp]:
-  "armKSASIDTable (armKSKernelVSpace_update f v) = armKSASIDTable v"
-  by (cases v) simp
-
-lemma armKSASIDTable_armKSGlobalPTs_update [simp]:
-  "armKSASIDTable (armKSGlobalPTs_update f v) = armKSASIDTable v"
-  by (cases v) simp
-
-lemma armKSASIDTable_armKSNextASID_update [simp]:
-  "armKSASIDTable (armKSNextASID_update f v) = armKSASIDTable v"
-  by (cases v) simp
-
-lemma armKSASIDTable_armKSASIDMap_update [simp]:
-  "armKSASIDTable (armKSASIDMap_update f v) = armKSASIDTable v"
-  by (cases v) simp
-
-lemma armKSGlobalPD_armKSGlobalsFrame_update [simp]:
-  "armKSGlobalPD (armKSGlobalsFrame_update f v) = armKSGlobalPD v"
-  by (cases v) simp
-
-lemma armKSGlobalPD_armKSASIDTable_update [simp]:
-  "armKSGlobalPD (armKSASIDTable_update f v) = armKSGlobalPD v"
-  by (cases v) simp
-
-lemma armKSGlobalPD_armKSGlobalPD_update [simp]:
-  "armKSGlobalPD (armKSGlobalPD_update f v) = f (armKSGlobalPD v)"
-  by (cases v) simp
-
-lemma armKSGlobalPD_armKSHWASIDTable_update [simp]:
-  "armKSGlobalPD (armKSHWASIDTable_update f v) = armKSGlobalPD v"
-  by (cases v) simp
-
-lemma armKSGlobalPD_armKSKernelVSpace_update [simp]:
-  "armKSGlobalPD (armKSKernelVSpace_update f v) = armKSGlobalPD v"
-  by (cases v) simp
-
-lemma armKSGlobalPD_armKSGlobalPTs_update [simp]:
-  "armKSGlobalPD (armKSGlobalPTs_update f v) = armKSGlobalPD v"
-  by (cases v) simp
-
-lemma armKSGlobalPD_armKSNextASID_update [simp]:
-  "armKSGlobalPD (armKSNextASID_update f v) = armKSGlobalPD v"
-  by (cases v) simp
-
-lemma armKSGlobalPD_armKSASIDMap_update [simp]:
-  "armKSGlobalPD (armKSASIDMap_update f v) = armKSGlobalPD v"
-  by (cases v) simp
-
-lemma armKSHWASIDTable_armKSGlobalsFrame_update [simp]:
-  "armKSHWASIDTable (armKSGlobalsFrame_update f v) = armKSHWASIDTable v"
-  by (cases v) simp
-
-lemma armKSHWASIDTable_armKSASIDTable_update [simp]:
-  "armKSHWASIDTable (armKSASIDTable_update f v) = armKSHWASIDTable v"
-  by (cases v) simp
-
-lemma armKSHWASIDTable_armKSGlobalPD_update [simp]:
-  "armKSHWASIDTable (armKSGlobalPD_update f v) = armKSHWASIDTable v"
-  by (cases v) simp
-
-lemma armKSHWASIDTable_armKSHWASIDTable_update [simp]:
-  "armKSHWASIDTable (armKSHWASIDTable_update f v) = f (armKSHWASIDTable v)"
-  by (cases v) simp
-
-lemma armKSHWASIDTable_armKSKernelVSpace_update [simp]:
-  "armKSHWASIDTable (armKSKernelVSpace_update f v) = armKSHWASIDTable v"
-  by (cases v) simp
-
-lemma armKSHWASIDTable_armKSGlobalPTs_update [simp]:
-  "armKSHWASIDTable (armKSGlobalPTs_update f v) = armKSHWASIDTable v"
-  by (cases v) simp
-
-lemma armKSHWASIDTable_armKSNextASID_update [simp]:
-  "armKSHWASIDTable (armKSNextASID_update f v) = armKSHWASIDTable v"
-  by (cases v) simp
-
-lemma armKSHWASIDTable_armKSASIDMap_update [simp]:
-  "armKSHWASIDTable (armKSASIDMap_update f v) = armKSHWASIDTable v"
-  by (cases v) simp
-
-lemma armKSKernelVSpace_armKSGlobalsFrame_update [simp]:
-  "armKSKernelVSpace (armKSGlobalsFrame_update f v) = armKSKernelVSpace v"
+lemma armKSKernelVSpace_armKSKernelVSpace_update [simp]:
+  "armKSKernelVSpace (armKSKernelVSpace_update f v) = f (armKSKernelVSpace v)"
   by (cases v) simp
 
 lemma armKSKernelVSpace_armKSASIDTable_update [simp]:
@@ -256,10 +118,6 @@ lemma armKSKernelVSpace_armKSHWASIDTable_update [simp]:
   "armKSKernelVSpace (armKSHWASIDTable_update f v) = armKSKernelVSpace v"
   by (cases v) simp
 
-lemma armKSKernelVSpace_armKSKernelVSpace_update [simp]:
-  "armKSKernelVSpace (armKSKernelVSpace_update f v) = f (armKSKernelVSpace v)"
-  by (cases v) simp
-
 lemma armKSKernelVSpace_armKSGlobalPTs_update [simp]:
   "armKSKernelVSpace (armKSGlobalPTs_update f v) = armKSKernelVSpace v"
   by (cases v) simp
@@ -272,8 +130,92 @@ lemma armKSKernelVSpace_armKSASIDMap_update [simp]:
   "armKSKernelVSpace (armKSASIDMap_update f v) = armKSKernelVSpace v"
   by (cases v) simp
 
-lemma armKSGlobalPTs_armKSGlobalsFrame_update [simp]:
-  "armKSGlobalPTs (armKSGlobalsFrame_update f v) = armKSGlobalPTs v"
+lemma armKSASIDTable_armKSKernelVSpace_update [simp]:
+  "armKSASIDTable (armKSKernelVSpace_update f v) = armKSASIDTable v"
+  by (cases v) simp
+
+lemma armKSASIDTable_armKSASIDTable_update [simp]:
+  "armKSASIDTable (armKSASIDTable_update f v) = f (armKSASIDTable v)"
+  by (cases v) simp
+
+lemma armKSASIDTable_armKSGlobalPD_update [simp]:
+  "armKSASIDTable (armKSGlobalPD_update f v) = armKSASIDTable v"
+  by (cases v) simp
+
+lemma armKSASIDTable_armKSHWASIDTable_update [simp]:
+  "armKSASIDTable (armKSHWASIDTable_update f v) = armKSASIDTable v"
+  by (cases v) simp
+
+lemma armKSASIDTable_armKSGlobalPTs_update [simp]:
+  "armKSASIDTable (armKSGlobalPTs_update f v) = armKSASIDTable v"
+  by (cases v) simp
+
+lemma armKSASIDTable_armKSNextASID_update [simp]:
+  "armKSASIDTable (armKSNextASID_update f v) = armKSASIDTable v"
+  by (cases v) simp
+
+lemma armKSASIDTable_armKSASIDMap_update [simp]:
+  "armKSASIDTable (armKSASIDMap_update f v) = armKSASIDTable v"
+  by (cases v) simp
+
+lemma armKSGlobalPD_armKSKernelVSpace_update [simp]:
+  "armKSGlobalPD (armKSKernelVSpace_update f v) = armKSGlobalPD v"
+  by (cases v) simp
+
+lemma armKSGlobalPD_armKSASIDTable_update [simp]:
+  "armKSGlobalPD (armKSASIDTable_update f v) = armKSGlobalPD v"
+  by (cases v) simp
+
+lemma armKSGlobalPD_armKSGlobalPD_update [simp]:
+  "armKSGlobalPD (armKSGlobalPD_update f v) = f (armKSGlobalPD v)"
+  by (cases v) simp
+
+lemma armKSGlobalPD_armKSHWASIDTable_update [simp]:
+  "armKSGlobalPD (armKSHWASIDTable_update f v) = armKSGlobalPD v"
+  by (cases v) simp
+
+lemma armKSGlobalPD_armKSGlobalPTs_update [simp]:
+  "armKSGlobalPD (armKSGlobalPTs_update f v) = armKSGlobalPD v"
+  by (cases v) simp
+
+lemma armKSGlobalPD_armKSNextASID_update [simp]:
+  "armKSGlobalPD (armKSNextASID_update f v) = armKSGlobalPD v"
+  by (cases v) simp
+
+lemma armKSGlobalPD_armKSASIDMap_update [simp]:
+  "armKSGlobalPD (armKSASIDMap_update f v) = armKSGlobalPD v"
+  by (cases v) simp
+
+lemma armKSHWASIDTable_armKSKernelVSpace_update [simp]:
+  "armKSHWASIDTable (armKSKernelVSpace_update f v) = armKSHWASIDTable v"
+  by (cases v) simp
+
+lemma armKSHWASIDTable_armKSASIDTable_update [simp]:
+  "armKSHWASIDTable (armKSASIDTable_update f v) = armKSHWASIDTable v"
+  by (cases v) simp
+
+lemma armKSHWASIDTable_armKSGlobalPD_update [simp]:
+  "armKSHWASIDTable (armKSGlobalPD_update f v) = armKSHWASIDTable v"
+  by (cases v) simp
+
+lemma armKSHWASIDTable_armKSHWASIDTable_update [simp]:
+  "armKSHWASIDTable (armKSHWASIDTable_update f v) = f (armKSHWASIDTable v)"
+  by (cases v) simp
+
+lemma armKSHWASIDTable_armKSGlobalPTs_update [simp]:
+  "armKSHWASIDTable (armKSGlobalPTs_update f v) = armKSHWASIDTable v"
+  by (cases v) simp
+
+lemma armKSHWASIDTable_armKSNextASID_update [simp]:
+  "armKSHWASIDTable (armKSNextASID_update f v) = armKSHWASIDTable v"
+  by (cases v) simp
+
+lemma armKSHWASIDTable_armKSASIDMap_update [simp]:
+  "armKSHWASIDTable (armKSASIDMap_update f v) = armKSHWASIDTable v"
+  by (cases v) simp
+
+lemma armKSGlobalPTs_armKSKernelVSpace_update [simp]:
+  "armKSGlobalPTs (armKSKernelVSpace_update f v) = armKSGlobalPTs v"
   by (cases v) simp
 
 lemma armKSGlobalPTs_armKSASIDTable_update [simp]:
@@ -288,10 +230,6 @@ lemma armKSGlobalPTs_armKSHWASIDTable_update [simp]:
   "armKSGlobalPTs (armKSHWASIDTable_update f v) = armKSGlobalPTs v"
   by (cases v) simp
 
-lemma armKSGlobalPTs_armKSKernelVSpace_update [simp]:
-  "armKSGlobalPTs (armKSKernelVSpace_update f v) = armKSGlobalPTs v"
-  by (cases v) simp
-
 lemma armKSGlobalPTs_armKSGlobalPTs_update [simp]:
   "armKSGlobalPTs (armKSGlobalPTs_update f v) = f (armKSGlobalPTs v)"
   by (cases v) simp
@@ -304,8 +242,8 @@ lemma armKSGlobalPTs_armKSASIDMap_update [simp]:
   "armKSGlobalPTs (armKSASIDMap_update f v) = armKSGlobalPTs v"
   by (cases v) simp
 
-lemma armKSNextASID_armKSGlobalsFrame_update [simp]:
-  "armKSNextASID (armKSGlobalsFrame_update f v) = armKSNextASID v"
+lemma armKSNextASID_armKSKernelVSpace_update [simp]:
+  "armKSNextASID (armKSKernelVSpace_update f v) = armKSNextASID v"
   by (cases v) simp
 
 lemma armKSNextASID_armKSASIDTable_update [simp]:
@@ -320,10 +258,6 @@ lemma armKSNextASID_armKSHWASIDTable_update [simp]:
   "armKSNextASID (armKSHWASIDTable_update f v) = armKSNextASID v"
   by (cases v) simp
 
-lemma armKSNextASID_armKSKernelVSpace_update [simp]:
-  "armKSNextASID (armKSKernelVSpace_update f v) = armKSNextASID v"
-  by (cases v) simp
-
 lemma armKSNextASID_armKSGlobalPTs_update [simp]:
   "armKSNextASID (armKSGlobalPTs_update f v) = armKSNextASID v"
   by (cases v) simp
@@ -336,8 +270,8 @@ lemma armKSNextASID_armKSASIDMap_update [simp]:
   "armKSNextASID (armKSASIDMap_update f v) = armKSNextASID v"
   by (cases v) simp
 
-lemma armKSASIDMap_armKSGlobalsFrame_update [simp]:
-  "armKSASIDMap (armKSGlobalsFrame_update f v) = armKSASIDMap v"
+lemma armKSASIDMap_armKSKernelVSpace_update [simp]:
+  "armKSASIDMap (armKSKernelVSpace_update f v) = armKSASIDMap v"
   by (cases v) simp
 
 lemma armKSASIDMap_armKSASIDTable_update [simp]:
@@ -350,10 +284,6 @@ lemma armKSASIDMap_armKSGlobalPD_update [simp]:
 
 lemma armKSASIDMap_armKSHWASIDTable_update [simp]:
   "armKSASIDMap (armKSHWASIDTable_update f v) = armKSASIDMap v"
-  by (cases v) simp
-
-lemma armKSASIDMap_armKSKernelVSpace_update [simp]:
-  "armKSASIDMap (armKSKernelVSpace_update f v) = armKSASIDMap v"
   by (cases v) simp
 
 lemma armKSASIDMap_armKSGlobalPTs_update [simp]:
@@ -384,7 +314,6 @@ where
             [globalPTs, globalPTs + bit pageBits  .e.  globalPTsTop - 1] @
             [globalPD, globalPD + bit pageBits  .e.  globalPDTop - 1];
         state = ARMKernelState_ \<lparr>
-            armKSGlobalsFrame= ptrFromPAddr globalsFrame,
             armKSASIDTable= funPartialArray (const Nothing) (0, (1 `~shiftL~` asidHighBits) - 1),
             armKSHWASIDTable= funArray (const Nothing),
             armKSNextASID= minBound,
